qstar/examples/Teleport.qs
@@ -1,0 +1,32 @@
+namespace QStar.Translator.Teleport {
+    open Microsoft.Quantum.Intrinsic;
+    open Microsoft.Quantum.Canon;
+
+    operation Entangle (qAlice : Qubit, qBob : Qubit)
+    : Unit is Adj {
+        H(qAlice);
+        CNOT(qAlice, qBob);
+    }
+
+    operation SendMsg (qAlice : Qubit, qMsg : Qubit)
+    : (Bool, Bool) {
+        Adjoint Entangle(qMsg, qAlice);
+        let m1 = M(qMsg);
+        let m2 = M(qAlice);
+        return (m1 == One, m2 == One);
+    }
+
+    operation DecodeMsg (qBob : Qubit, (b1 : Bool, b2 : Bool))
+    : Unit {
+        if b1 { Z(qBob); }
+        if b2 { X(qBob); }
+    }
+
+    operation Teleport (qAlice : Qubit, qBob : Qubit)
+    : Unit {
+        use qMsg = Qubit();
+        Entangle(qAlice, qBob);
+        let classicalBits = SendMsg(qAlice, qMsg);
+        DecodeMsg(qBob, classicalBits);
+    }
+}
